second version of append to simplify simulation definitions

src/computational_monads/simulation_semantics/constructions/counting_oracle.lean
@@ -15,12 +15,20 @@ variables {α β γ : Type} {spec spec' : oracle_spec}
   (oa : oracle_comp spec α) (ob : α → oracle_comp spec β) (n m : ℕ)
 
 /-- Simulation oracle that just counts the number of queries to the oracles -/
-def counting_oracle : simulation_oracle spec spec :=
+def counting_oracle (spec : oracle_spec) : simulation_oracle spec spec :=
 ⟪ query | λ n _ _ _, n + 1 , 0 ⟫
 
 namespace counting_oracle
 
+lemma apply (i : spec.ι) (t : spec.domain i) (n : ℕ) :
+  (counting_oracle spec).o i (t, n) = do { u ← query i t, pure (u, (n + 1 : ℕ)) } := rfl
+
 section support
+
+lemma support_apply (i : spec.ι) (t : spec.domain i) (n : ℕ) :
+  ((counting_oracle spec).o i (t, n)).support = {x | x.2 = nat.succ n} :=
+(tracking_oracle.support_apply query _ _ i t n).trans
+  (by simpa only [support_query, set.top_eq_univ, set.mem_univ, true_and])
 
 end support
 
